proof of pavx2 done

proof/crypto_stream/chacha20/ref/ChaCha20_avx2_pv.ec
@@ -35,7 +35,7 @@ module M = {
     k <- st;
     return (k);
   }
-*)  
+
   proc sum_states (k:W32.t Array16.t, st:W32.t Array16.t) : W32.t Array16.t = {
     var aux: int;
     
@@ -49,6 +49,8 @@ module M = {
     return (k);
   }
   
+*)  
+
   proc update_ptr (output:W64.t, plain:W64.t, len:W32.t, n:int) : W64.t *
                                                                   W64.t *
                                                                   W32.t = {
@@ -247,106 +249,70 @@ module M = {
     
     var k, st1:W32.t Array16.t;
     k <@ ChaCha20_pref.M.rounds (st);
-    k <@ sum_states (k, st);
+    k <@ ChaCha20_pref.M.sum_states (k, st);
     st1 <@ ChaCha20_pref.M.increment_counter (st);
     return (k, st1);
   }
   
+  proc body_x8(st_1: W32.t Array16.t) = {
+    var st_2, st_3, st_4, st_5, st_6, st_7, st_8 : W32.t Array16.t;
+    var k_1, k_2, k_3, k_4, k_5, k_6, k_7, k_8 : W32.t Array16.t;
+
+    k_1 <@ ChaCha20_pref.M.rounds (st_1);
+    k_1 <@ ChaCha20_pref.M.sum_states (k_1, st_1);
+    st_2 <@ ChaCha20_pref.M.increment_counter (st_1);
+
+    k_2 <@ ChaCha20_pref.M.rounds (st_2);
+    k_2 <@ ChaCha20_pref.M.sum_states (k_2, st_2);
+    st_3 <@ ChaCha20_pref.M.increment_counter (st_2);
+  
+    k_3 <@ ChaCha20_pref.M.rounds (st_3);
+    k_3 <@ ChaCha20_pref.M.sum_states (k_3, st_3);
+    st_4 <@ ChaCha20_pref.M.increment_counter (st_3);
+
+    k_4 <@ ChaCha20_pref.M.rounds (st_4);
+    k_4 <@ ChaCha20_pref.M.sum_states (k_4, st_4);
+    st_5 <@ ChaCha20_pref.M.increment_counter (st_4);
+
+    k_5 <@ ChaCha20_pref.M.rounds (st_5);
+    k_5 <@ ChaCha20_pref.M.sum_states (k_5, st_5);
+    st_6 <@ ChaCha20_pref.M.increment_counter (st_5);
+
+    k_6 <@ ChaCha20_pref.M.rounds (st_6);
+    k_6 <@ ChaCha20_pref.M.sum_states (k_6, st_6);
+    st_7 <@ ChaCha20_pref.M.increment_counter (st_6);
+  
+    k_7 <@ ChaCha20_pref.M.rounds (st_7);
+    k_7 <@ ChaCha20_pref.M.sum_states (k_7, st_7);
+    st_8 <@ ChaCha20_pref.M.increment_counter (st_7);
+
+    k_8 <@ ChaCha20_pref.M.rounds (st_8);
+    k_8 <@ ChaCha20_pref.M.sum_states (k_8, st_8);
+    st_1 <@ ChaCha20_pref.M.increment_counter (st_8);
+    return (st_1, k_1, k_2, k_3, k_4, k_5, k_6, k_7, k_8);
+  }
+     
   proc chacha20_more_than_256 (output:W64.t, plain:W64.t, len:W32.t,
                                key:W64.t, nonce:W64.t, counter:W32.t) : unit = {
     
     var st_1:W32.t Array16.t;
-    var k_1:W32.t Array16.t;
-    var st_2:W32.t Array16.t;
-    var k_2:W32.t Array16.t;
-    var st_3:W32.t Array16.t;
-    var k_3:W32.t Array16.t;
-    var st_4:W32.t Array16.t;
-    var k_4:W32.t Array16.t;
-    var st_5:W32.t Array16.t;
-    var k_5:W32.t Array16.t;
-    var st_6:W32.t Array16.t;
-    var k_6:W32.t Array16.t;
-    var st_7:W32.t Array16.t;
-    var k_7:W32.t Array16.t;
-    var st_8:W32.t Array16.t;
-    var k_8:W32.t Array16.t;
+    var k_1, k_2, k_3, k_4, k_5, k_6, k_7, k_8 : W32.t Array16.t;
 
     st_1 <@ ChaCha20_pref.M.init (key, nonce, counter);
     
-    while (((W32.of_int 512) \ule len)) {
-      k_1 <@ ChaCha20_pref.M.rounds (st_1);
-      k_1 <@ sum_states (k_1, st_1);
-      st_2 <@ ChaCha20_pref.M.increment_counter (st_1);
-
-      k_2 <@ ChaCha20_pref.M.rounds (st_2);
-      k_2 <@ sum_states (k_2, st_2);
-      st_3 <@ ChaCha20_pref.M.increment_counter (st_2);
-  
-      k_3 <@ ChaCha20_pref.M.rounds (st_3);
-      k_3 <@ sum_states (k_3, st_3);
-      st_4 <@ ChaCha20_pref.M.increment_counter (st_3);
-
-      k_4 <@ ChaCha20_pref.M.rounds (st_4);
-      k_4 <@ sum_states (k_4, st_4);
-      st_5 <@ ChaCha20_pref.M.increment_counter (st_4);
-
-      k_5 <@ ChaCha20_pref.M.rounds (st_5);
-      k_5 <@ sum_states (k_5, st_5);
-      st_6 <@ ChaCha20_pref.M.increment_counter (st_6);
-
-      k_6 <@ ChaCha20_pref.M.rounds (st_6);
-      k_6 <@ sum_states (k_6, st_6);
-      st_7 <@ ChaCha20_pref.M.increment_counter (st_7);
-  
-      k_7 <@ ChaCha20_pref.M.rounds (st_7);
-      k_7 <@ sum_states (k_7, st_7);
-      st_8 <@ ChaCha20_pref.M.increment_counter (st_7);
-
-      k_8 <@ ChaCha20_pref.M.rounds (st_8);
-      k_8 <@ sum_states (k_8, st_8);
-      st_1 <@ ChaCha20_pref.M.increment_counter (st_8);
-
+    while (W32.of_int 512 \ule len) {
+      (st_1, k_1, k_2, k_3, k_4, k_5, k_6, k_7, k_8) <- body_x8(st_1);
       (output, plain, len) <@ store_x8 (output, plain, len, k_1, k_2, k_3, k_4, k_5, k_6, k_7, k_8);
     }
-    if (((W32.of_int 0) \ult len)) {
-      k_1 <@ ChaCha20_pref.M.rounds (st_1);
-      k_1 <@ sum_states (k_1, st_1);
-      st_2 <@ ChaCha20_pref.M.increment_counter (st_1);
-
-      k_2 <@ ChaCha20_pref.M.rounds (st_2);
-      k_2 <@ sum_states (k_2, st_2);
-      st_3 <@ ChaCha20_pref.M.increment_counter (st_2);
-  
-      k_3 <@ ChaCha20_pref.M.rounds (st_3);
-      k_3 <@ sum_states (k_3, st_3);
-      st_4 <@ ChaCha20_pref.M.increment_counter (st_3);
-
-      k_4 <@ ChaCha20_pref.M.rounds (st_4);
-      k_4 <@ sum_states (k_4, st_4);
-      st_5 <@ ChaCha20_pref.M.increment_counter (st_4);
-
-      k_5 <@ ChaCha20_pref.M.rounds (st_5);
-      k_5 <@ sum_states (k_5, st_5);
-      st_6 <@ ChaCha20_pref.M.increment_counter (st_6);
-
-      k_6 <@ ChaCha20_pref.M.rounds (st_6);
-      k_6 <@ sum_states (k_6, st_6);
-      st_7 <@ ChaCha20_pref.M.increment_counter (st_7);
-  
-      k_7 <@ ChaCha20_pref.M.rounds (st_7);
-      k_7 <@ sum_states (k_7, st_7);
-      st_8 <@ ChaCha20_pref.M.increment_counter (st_7);
-
-      k_8 <@ ChaCha20_pref.M.rounds (st_8);
-      k_8 <@ sum_states (k_8, st_8);
+    if (W32.of_int 0 \ult len) {
+      (st_1, k_1, k_2, k_3, k_4, k_5, k_6, k_7, k_8) <- body_x8(st_1);
       store_x8_last (output, plain, len, k_1, k_2, k_3, k_4, k_5, k_6, k_7, k_8);
     } 
   }
 
   proc chacha20_ref_loop (output:W64.t, plain:W64.t, len:W32.t, st : W32.t Array16.t) : unit = {
      var k:W32.t Array16.t;
-     while (((W32.of_int 0) \ult len)) {
+     while (W32.of_int 0 \ult len) {
       (k, st) <@ chacha20_body(st);
       (output, plain, len) <@ ChaCha20_pref.M.store (output, plain, len, k);
     }
@@ -364,11 +330,11 @@ module M = {
     var k_1, k_2, st_2 :W32.t Array16.t;
       
     k_1 <@ ChaCha20_pref.M.rounds (st_1);
-    k_1 <@ sum_states (k_1, st_1);
+    k_1 <@ ChaCha20_pref.M.sum_states (k_1, st_1);
     st_2 <@ ChaCha20_pref.M.increment_counter (st_1);
 
     k_2 <@ ChaCha20_pref.M.rounds (st_2);
-    k_2 <@ sum_states (k_2, st_2);
+    k_2 <@ ChaCha20_pref.M.sum_states (k_2, st_2);
 (*    st_3 <@ ChaCha20_pref.M.increment_counter (st_2); *)
 
     store_x2_last (output, plain, len, k_1, k_2);
@@ -378,22 +344,22 @@ module M = {
     var k_1, k_2, k_3, k_4, st_2, st_3, st_4 : W32.t Array16.t;
 
     k_1 <@ ChaCha20_pref.M.rounds (st_1);
-    k_1 <@ sum_states (k_1, st_1);
+    k_1 <@ ChaCha20_pref.M.sum_states (k_1, st_1);
     st_2 <@ ChaCha20_pref.M.increment_counter (st_1);
 
     k_2 <@ ChaCha20_pref.M.rounds (st_2);
-    k_2 <@ sum_states (k_2, st_2);
+    k_2 <@ ChaCha20_pref.M.sum_states (k_2, st_2);
     st_3 <@ ChaCha20_pref.M.increment_counter (st_2);
   
     k_3 <@ ChaCha20_pref.M.rounds (st_3);
-    k_3 <@ sum_states (k_3, st_3);
+    k_3 <@ ChaCha20_pref.M.sum_states (k_3, st_3);
     st_4 <@ ChaCha20_pref.M.increment_counter (st_3);
 
     k_4 <@ ChaCha20_pref.M.rounds (st_4);
-    k_4 <@ sum_states (k_4, st_4);
+    k_4 <@ ChaCha20_pref.M.sum_states (k_4, st_4);
 
     (output, plain, len) <@ store_x2 (output, plain, len, k_1, k_2);
-    store_x2_last (output, plain, len, k_1, k_2);
+    store_x2_last (output, plain, len, k_3, k_4);
 
   }
 
