proof/crypto_stream/chacha20/ref/ChaCha20_pavx2.ec
@@ -1,7 +1,31 @@
 require import List Jasmin_model Int IntDiv CoreMap.
-require import Array16.
+require import Array8 Array16.
 require import WArray64.
 require import ChaCha20_pref ChaCha20_avx2_pv.
+
+(*
+(* Merge this with Ops poly *)
+type t8u32 = W32.t Array8.t.
+
+module Ops = {
+  proc ivadd8u32(x y:t8u32) : t8u32 = {
+    var r : t8u32;
+    r.[0] <- x.[0] + y.[0];
+    r.[1] <- x.[1] + y.[1];
+    r.[2] <- x.[2] + y.[2];
+    r.[3] <- x.[3] + y.[3];
+    return r; 
+  }
+
+  proc ixor8u32 (x y:t8u32) : t8u32 = {
+    var r : t4u64;
+    r.[0] <- x.[0] `^` y.[0];
+    r.[1] <- x.[1] `^` y.[1];
+    r.[2] <- x.[2] `^` y.[2];
+    r.[3] <- x.[3] `^` y.[3];
+    return r;
+  }
+*)
 
 module M = {
   proc init_x2(key:W64.t, nonce:W64.t, counter:W32.t) : W32.t Array16.t * W32.t Array16.t = {
@@ -11,24 +35,135 @@ module M = {
     return (st_1, st_2);
   }
 
-  proc column_round_x2(k1_1 k1_2: W32.t Array16.t) : W32.t Array16.t * W32.t Array16.t = {
-    k1_1 <@  ChaCha20_pref.M.column_round(k1_1);
-    k1_2 <@  ChaCha20_pref.M.column_round(k1_2);
-    return (k1_1, k1_2);
+  proc line_x4 (k: W32.t Array16.t, a b c r: int) : W32.t Array16.t = {
+    var i : int;
+    k.[a + 0] <- k.[a + 0] + k.[b + 0];
+    k.[a + 1] <- k.[a + 1] + k.[b + 1];
+    k.[a + 2] <- k.[a + 2] + k.[b + 2];
+    k.[a + 3] <- k.[a + 3] + k.[b + 3];
+
+    k.[c + 0] <- k.[c + 0] `^` k.[a + 0];
+    k.[c + 1] <- k.[c + 1] `^` k.[a + 1];
+    k.[c + 2] <- k.[c + 2] `^` k.[a + 2];
+    k.[c + 3] <- k.[c + 3] `^` k.[a + 3];
+
+    k.[c + 0] <- rol k.[c + 0] r;
+    k.[c + 1] <- rol k.[c + 1] r;
+    k.[c + 2] <- rol k.[c + 2] r;
+    k.[c + 3] <- rol k.[c + 3] r;
+
+    return k;
   }
 
-  proc diagonal_round_x2(k1_1 k1_2: W32.t Array16.t) : W32.t Array16.t * W32.t Array16.t = {
-    k1_1 <@  ChaCha20_pref.M.diagonal_round(k1_1);
-    k1_2 <@  ChaCha20_pref.M.diagonal_round(k1_2);
-    return (k1_1, k1_2);
+  proc column_round(k: W32.t Array16.t) : W32.t Array16.t = {
+    k <@ line_x4(k, 0, 4, 12, 16);
+    k <@ line_x4(k, 8, 12, 4, 12);
+    k <@ line_x4(k, 0, 4, 12,  8);
+    k <@ line_x4(k, 8, 12, 4,  7);
+    return k;
   }
 
-  proc rounds_x2_aux(k1_1 k1_2: W32.t Array16.t) : W32.t Array16.t * W32.t Array16.t = {
-    k1_1 <@ ChaCha20_pref.M.rounds(k1_1);
-    k1_2 <@ ChaCha20_pref.M.rounds(k1_2);
-    return (k1_1, k1_2);
+  proc shuffle_state_1 (k: W32.t Array16.t) : W32.t Array16.t = {
+    var k' : W32.t Array16.t;
+
+    k'.[0]  <- k.[0] ;
+    k'.[1]  <- k.[1] ;
+    k'.[2]  <- k.[2] ;
+    k'.[3]  <- k.[3] ;
+ 
+    k'.[4]  <- k.[5] ;
+    k'.[5]  <- k.[6] ;
+    k'.[6]  <- k.[7] ;
+    k'.[7]  <- k.[4] ;
+
+    k'.[8]  <- k.[10];
+    k'.[9]  <- k.[11];
+    k'.[10] <- k.[8] ;
+    k'.[11] <- k.[9] ;
+
+    k'.[12] <- k.[15];
+    k'.[13] <- k.[12];
+    k'.[14] <- k.[13];
+    k'.[15] <- k.[14];
+    return k';
   }
 
+  proc reverse_shuffle_state_1 (k: W32.t Array16.t) : W32.t Array16.t = {
+    var k' : W32.t Array16.t;
+
+    k'.[0]  <- k.[0] ;
+    k'.[1]  <- k.[1] ;
+    k'.[2]  <- k.[2] ;
+    k'.[3]  <- k.[3] ;
+
+    k'.[5]  <- k.[4] ;
+    k'.[6]  <- k.[5] ;
+    k'.[7]  <- k.[6] ;
+    k'.[4]  <- k.[7] ;
+
+    k'.[10] <- k.[8] ;
+    k'.[11] <- k.[9] ;
+    k'.[8]  <- k.[10];
+    k'.[9]  <- k.[11];
+
+    k'.[15] <- k.[12];
+    k'.[12] <- k.[13];
+    k'.[13] <- k.[14];
+    k'.[14] <- k.[15];
+    return k';
+  }
+
+  proc diagonal_round(k: W32.t Array16.t) : W32.t Array16.t = {
+    k <@ shuffle_state_1(k);
+    k <@ column_round(k);
+    k <@ reverse_shuffle_state_1(k);
+    return k;
+  }
+
+  proc rounds(k: W32.t Array16.t) : W32.t Array16.t = {
+    var c : int;
+    c <- 0;
+    while (c < 10) {
+      k <- column_round(k);
+      k <- diagonal_round(k);
+      c <- c + 1;
+    }
+    return k;
+  }
+
+  proc line_x8(k1 k2: W32.t Array16.t, a b c r:int) : W32.t Array16.t * W32.t Array16.t = {
+    k1 <@ line_x4(k1, a, b, c, r);
+    k2 <@ line_x4(k2, a, b, c, r);
+    return (k1,k2);
+  }
+
+  proc column_round_x2(k1 k2: W32.t Array16.t) : W32.t Array16.t * W32.t Array16.t = {
+    (k1,k2) <@ line_x8(k1, k2, 0, 4, 12, 16);
+    (k1,k2) <@ line_x8(k1, k2, 8, 12, 4, 12);
+    (k1,k2) <@ line_x8(k1, k2, 0, 4, 12,  8);
+    (k1,k2) <@ line_x8(k1, k2, 8, 12, 4,  7);
+    return (k1, k2);
+  }
+
+  proc shuffle_state(k1 k2: W32.t Array16.t) : W32.t Array16.t * W32.t Array16.t = {
+    k1 <@ shuffle_state_1(k1);
+    k2 <@ shuffle_state_1(k2);
+    return (k1, k2);
+  }
+
+  proc reverse_shuffle_state(k1 k2: W32.t Array16.t) : W32.t Array16.t * W32.t Array16.t = {
+    k1 <@ reverse_shuffle_state_1(k1);
+    k2 <@ reverse_shuffle_state_1(k2);
+    return (k1, k2);
+  }
+
+  proc diagonal_round_x2(k1 k2: W32.t Array16.t) : W32.t Array16.t * W32.t Array16.t = {
+    (k1, k2) <@ shuffle_state(k1, k2);
+    (k1, k2) <@ column_round_x2(k1, k2);
+    (k1, k2) <@ reverse_shuffle_state(k1, k2);
+    return (k1, k2);
+  }
+  
   proc rounds_x2(k1_1 k1_2: W32.t Array16.t) : W32.t Array16.t * W32.t Array16.t = {
     var c : int;
     c <- 0;
@@ -37,6 +172,25 @@ module M = {
       (k1_1, k1_2) <- diagonal_round_x2(k1_1, k1_2);
       c <- c + 1;
     }
+    return (k1_1, k1_2);
+  }
+
+  proc column_round_x2_aux(k1_1 k1_2: W32.t Array16.t) : W32.t Array16.t * W32.t Array16.t = {
+    k1_1 <@  column_round(k1_1);
+    k1_2 <@  column_round(k1_2);
+    return (k1_1, k1_2);
+  }
+
+(*
+  proc diagonal_round_x2_aux(k1_1 k1_2: W32.t Array16.t) : W32.t Array16.t * W32.t Array16.t = {
+    k1_1 <@  ChaCha20_pref.M.diagonal_round(k1_1);
+    k1_2 <@  ChaCha20_pref.M.diagonal_round(k1_2);
+    return (k1_1, k1_2);
+  } *)
+
+  proc rounds_x2_aux(k1_1 k1_2: W32.t Array16.t) : W32.t Array16.t * W32.t Array16.t = {
+    k1_1 <@ rounds(k1_1);
+    k1_2 <@ rounds(k1_2);
     return (k1_1, k1_2);
   }
 
@@ -53,10 +207,46 @@ module M = {
     return (st_1, st_2);
   }
 
-  proc rounds_x4 (st_1, st_2, st_3, st_4 :  W32.t Array16.t) = {
+ (* proc rounds_x4_aux (st_1, st_2, st_3, st_4 :  W32.t Array16.t) = {
     (st_1, st_2) <@ rounds_x2 (st_1, st_2);
     (st_3, st_4) <@ rounds_x2 (st_3, st_4);
     return (st_1, st_2, st_3, st_4);
+  }*)
+
+  proc column_round_x4 (k1_1 k1_2 k2_1 k2_2: W32.t Array16.t) = {
+    (k1_1, k1_2) = column_round_x2(k1_1, k1_2);
+    (k2_1, k2_2) = column_round_x2(k2_1, k2_2);
+    return (k1_1, k1_2, k2_1, k2_2);
+  }
+
+  proc shuffle_state_x2(k1_1 k1_2 k2_1 k2_2: W32.t Array16.t) = {
+    (k1_1, k1_2) = shuffle_state(k1_1, k1_2);
+    (k2_1, k2_2) = shuffle_state(k2_1, k2_2);
+    return (k1_1, k1_2, k2_1, k2_2);
+  }
+
+  proc reverse_shuffle_state_x2(k1_1 k1_2 k2_1 k2_2: W32.t Array16.t) = {
+    (k1_1, k1_2) = reverse_shuffle_state(k1_1, k1_2);
+    (k2_1, k2_2) = reverse_shuffle_state(k2_1, k2_2);
+    return (k1_1, k1_2, k2_1, k2_2);
+  }
+
+  proc diagonal_round_x4 (k1_1 k1_2 k2_1 k2_2: W32.t Array16.t) = {
+   (k1_1, k1_2, k2_1, k2_2) <@ shuffle_state_x2(k1_1, k1_2, k2_1, k2_2);
+   (k1_1, k1_2, k2_1, k2_2) <@ column_round_x4(k1_1, k1_2, k2_1, k2_2);
+   (k1_1, k1_2, k2_1, k2_2) <@ reverse_shuffle_state_x2(k1_1, k1_2, k2_1, k2_2);
+   return (k1_1, k1_2, k2_1, k2_2);
+  }
+
+  proc rounds_x4(k1_1 k1_2 k2_1 k2_2: W32.t Array16.t) = {
+    var c : int;
+    c <- 0;
+    while (c < 10) {
+      (k1_1, k1_2, k2_1, k2_2) <@ column_round_x4(k1_1, k1_2, k2_1, k2_2);
+      (k1_1, k1_2, k2_1, k2_2) <@ diagonal_round_x4(k1_1, k1_2, k2_1, k2_2);
+      c <- c + 1;
+    }
+    return (k1_1, k1_2, k2_1, k2_2);
   }
 
   proc sum_states_x4(k1_1 k1_2 k2_1 k2_2 st_1 st_2: W32.t Array16.t) = {
@@ -84,18 +274,227 @@ module M = {
     } 
   }
 
-  proc chacha20_more_than_256(output:W64.t, plain:W64.t, len:W32.t,
-                               key:W64.t, nonce:W64.t, counter:W32.t) : unit = {
+  (* ------------------------------------------------------------------- *)
+  (* more than 256                                                       *)
+
+  proc init_x8(key, nonce, counter) = {
+    var st_1 : W32.t Array16.t;
+    var st: W32.t Array16.t Array8.t;
+    st_1 <@ ChaCha20_pref.M.init (key, nonce, counter);
+    st.[0] <- st_1; 
+    st.[1] <- st_1.[12 <- st_1.[12] + W32.of_int 1];
+    st.[2] <- st_1.[12 <- st_1.[12] + W32.of_int 2];
+    st.[3] <- st_1.[12 <- st_1.[12] + W32.of_int 3];
+    st.[4] <- st_1.[12 <- st_1.[12] + W32.of_int 4];
+    st.[5] <- st_1.[12 <- st_1.[12] + W32.of_int 5];
+    st.[6] <- st_1.[12 <- st_1.[12] + W32.of_int 6];
+    st.[7] <- st_1.[12 <- st_1.[12] + W32.of_int 7];
+    return st; 
   }
 
+  proc sum_states_x8(k st: W32.t Array16.t Array8.t) = {
+    var i: int;
+    i <- 0;
+    while (i < 8) {
+      k.[i] <@ ChaCha20_pref.M.sum_states(k.[i], st.[i]);
+      i <- i + 1;
+    }
+    return k;
+  }
+
+  proc increment_counter_x8(st: W32.t Array16.t Array8.t) = {
+    var i: int;
+    i <- 0;
+    while (i < 8) {
+      st.[i] <- st.[i].[12 <- st.[i].[12] + W32.of_int 8];
+      i <- i + 1;
+    }
+    return st;
+  }    
+  
+  proc double_quarter_round_x1_aux (k: W32.t Array16.t, a0 b0 c0 d0 a1 b1 c1 d1 : int) = {
+    k <@ ChaCha20_pref.M.quarter_round(k, a0, b0, c0, d0);
+    k <@ ChaCha20_pref.M.quarter_round(k, a1, b1, c1, d1);
+    return k;
+  }
+
+  proc line_2 (k:W32.t Array16.t, a0 b0 c0 r0 a1 b1 c1 r1:int) = {
+    k.[a0] <- (k.[a0] + k.[b0]);
+    k.[a1] <- (k.[a1] + k.[b1]);
+
+    k.[c0] <- (k.[c0] `^` k.[a0]);
+    k.[c1] <- (k.[c1] `^` k.[a1]);
+
+    k.[c0] <- rol k.[c0] r0;
+    k.[c1] <- rol k.[c1] r1;
+
+    return (k);
+  }
+  
+  proc line_x1_8(k1 k2 k3 k4 k5 k6 k7 k8: W32.t Array16.t, a b c r: int) = {
+    k1 <@ ChaCha20_pref.M.line(k1, a, b, c, r);
+    k2 <@ ChaCha20_pref.M.line(k2, a, b, c, r);
+    k3 <@ ChaCha20_pref.M.line(k3, a, b, c, r);
+    k4 <@ ChaCha20_pref.M.line(k4, a, b, c, r);
+    k5 <@ ChaCha20_pref.M.line(k5, a, b, c, r);
+    k6 <@ ChaCha20_pref.M.line(k6, a, b, c, r);
+    k7 <@ ChaCha20_pref.M.line(k7, a, b, c, r);
+    k8 <@ ChaCha20_pref.M.line(k8, a, b, c, r);
+    return (k1,k2,k3,k4,k5,k6,k7,k8);
+  }
+
+  proc line_2_x1_8 (k1 k2 k3 k4 k5 k6 k7 k8: W32.t Array16.t, a0 b0 c0 r0 a1 b1 c1 r1 : int) = {
+    k1 <@ line_2(k1, a0, b0, c0, r0, a1, b1, c1, r1);
+    k2 <@ line_2(k2, a0, b0, c0, r0, a1, b1, c1, r1);
+    k3 <@ line_2(k3, a0, b0, c0, r0, a1, b1, c1, r1);
+    k4 <@ line_2(k4, a0, b0, c0, r0, a1, b1, c1, r1);
+    k5 <@ line_2(k5, a0, b0, c0, r0, a1, b1, c1, r1);
+    k6 <@ line_2(k6, a0, b0, c0, r0, a1, b1, c1, r1);
+    k7 <@ line_2(k7, a0, b0, c0, r0, a1, b1, c1, r1);
+    k8 <@ line_2(k8, a0, b0, c0, r0, a1, b1, c1, r1);
+    return (k1,k2,k3,k4,k5,k6,k7,k8);
+  }
+
+  proc double_quarter_round_x1 (k: W32.t Array16.t, a0 b0 c0 d0 a1 b1 c1 d1 : int) = {
+    k <@ ChaCha20_pref.M.line (k, a0, b0, d0, 16);
+    k <@ line_2(k, c0, d0, b0, 12, a1, b1, d1, 16);
+    k <@ line_2(k, a0, b0, d0, 8,  c1, d1, b1, 12);
+    k <@ line_2(k, c0, d0, b0, 7,  a1, b1, d1, 8);
+    k <@  ChaCha20_pref.M.line(k,  c1, d1, b1, 7);
+    return k;
+  }
+
+  proc double_quarter_round_x1_8 (k1 k2 k3 k4 k5 k6 k7 k8: W32.t Array16.t, a0 b0 c0 d0 a1 b1 c1 d1 : int) = {
+    k1 <@ double_quarter_round_x1(k1, a0, b0, c0, d0, a1, b1, c1, d1);
+    k2 <@ double_quarter_round_x1(k2, a0, b0, c0, d0, a1, b1, c1, d1);
+    k3 <@ double_quarter_round_x1(k3, a0, b0, c0, d0, a1, b1, c1, d1);
+    k4 <@ double_quarter_round_x1(k4, a0, b0, c0, d0, a1, b1, c1, d1);
+    k5 <@ double_quarter_round_x1(k5, a0, b0, c0, d0, a1, b1, c1, d1);
+    k6 <@ double_quarter_round_x1(k6, a0, b0, c0, d0, a1, b1, c1, d1);
+    k7 <@ double_quarter_round_x1(k7, a0, b0, c0, d0, a1, b1, c1, d1);
+    k8 <@ double_quarter_round_x1(k8, a0, b0, c0, d0, a1, b1, c1, d1);
+    return (k1,k2,k3,k4,k5,k6,k7,k8);
+  }
+
+  proc column_round_x1(k: W32.t Array16.t) = {
+    k <@ double_quarter_round_x1(k, 0, 4, 8,  12,     
+                                   2, 6, 10, 14);
+    k <@ double_quarter_round_x1(k, 1, 5, 9,  13,
+                                   3, 7, 11, 15);
+    return k;
+  }
+
+  proc diagonal_round_x1(k: W32.t Array16.t) = {
+    k <@ double_quarter_round_x1(k, 1, 6, 11, 12,
+                                    0, 5, 10, 15);
+    k <@ double_quarter_round_x1(k, 2, 7, 8, 13,
+                                    3, 4, 9, 14);
+    return k;
+  }
+
+  proc line_x8_v (k: W32.t Array16.t Array8.t , a b c r:int) = {
+    var i:int;
+    i <- 0; 
+    while (i < 8) {
+      k.[i] <@ ChaCha20_pref.M.line(k.[i], a, b, c, r);
+      i <- i + 1;
+    }
+    return k;
+  }
+
+  proc line_2_x8_v (k:W32.t Array16.t Array8.t, a0 b0 c0 r0 a1 b1 c1 r1:int) = {
+    var i:int;
+    i <- 0; 
+    while (i < 8) {
+      k.[i] <@ line_2(k.[i], a0, b0, c0, r0, a1, b1, c1, r1);
+      i <- i + 1;
+    }
+    return k;
+  }
+
+  proc double_quarter_round_x8 (k: W32.t Array16.t Array8.t, a0 b0 c0 d0 a1 b1 c1 d1 : int) = {
+    k <@ line_x8_v (k, a0, b0, d0, 16);
+    k <@ line_2_x8_v(k, c0, d0, b0, 12, a1, b1, d1, 16);
+    k <@ line_2_x8_v(k, a0, b0, d0, 8,  c1, d1, b1, 12);
+    k <@ line_2_x8_v(k, c0, d0, b0, 7,  a1, b1, d1, 8);
+    k <@ line_x8_v(k,  c1, d1, b1, 7);
+    return k;
+  }
+
+  proc column_round_x8(k: W32.t Array16.t Array8.t) = {
+    k <@ double_quarter_round_x8(k, 0, 4, 8,  12,     
+                                   2, 6, 10, 14);
+    k <@ double_quarter_round_x8(k, 1, 5, 9,  13,
+                                   3, 7, 11, 15);
+    return k;
+  }
+
+  proc diagonal_round_x8(k: W32.t Array16.t Array8.t) = {
+    k <@ double_quarter_round_x8(k, 1, 6, 11, 12,
+                                    0, 5, 10, 15);
+    k <@ double_quarter_round_x8(k, 2, 7, 8, 13,
+                                    3, 4, 9, 14);
+    return k;
+  }
+  
+  proc rounds_x1 (k: W32.t Array16.t) = {
+    var c : int;
+    c <- 0;
+    while (c < 10) {
+      k <@ column_round_x1(k);
+      k <@ diagonal_round_x1(k);
+      c <- c + 1;
+    }
+    return k;
+  }
+
+  proc rounds_x8 (k: W32.t Array16.t Array8.t) = {
+    var c : int;
+    c <- 0;
+    while (c < 10) {
+      k <@ column_round_x8(k);
+      k <@ diagonal_round_x8(k);
+      c <- c + 1;
+    }
+    return k;
+  }
+
+  proc body_x8 (st: W32.t Array16.t Array8.t) = {
+    var k: W32.t Array16.t Array8.t;
+    k <@ rounds_x8(st);
+    k <@ sum_states_x8(k, st);
+    st <@ increment_counter_x8(st);
+    return (k, st);
+  }
+
+  proc chacha20_more_than_256(output:W64.t, plain:W64.t, len:W32.t,
+                               key:W64.t, nonce:W64.t, counter:W32.t) : unit = {
+    var st, k: W32.t Array16.t Array8.t;
+    
+    st <@ init_x8(key, nonce, counter);
+
+    while( W32.of_int 512 \ule len) {
+      k <@ rounds_x8(st);
+      k <@ sum_states_x8(k, st);
+      (output, plain, len) <@ ChaCha20_avx2_pv.M.store_x8(output, plain, len, k.[0], k.[1], k.[2], k.[3],
+                                                                              k.[4], k.[5], k.[6], k.[7]);
+      st <@ increment_counter_x8(st);
+    }
+
+    if(W32.of_int 0 \ult len) {
+      k <@ rounds_x8(st);
+      k <@ sum_states_x8(k, st);
+      ChaCha20_avx2_pv.M.store_x8_last(output, plain, len, k.[0], k.[1], k.[2], k.[3],
+                                                      k.[4], k.[5], k.[6], k.[7]);
+    }
+  }
 
   proc chacha20_avx2(output:W64.t, plain:W64.t, len:W32.t,
                                key:W64.t, nonce:W64.t, counter:W32.t) : unit = {
     if (len \ult W32.of_int 257) {
       chacha20_less_than_257(output, plain, len, key, nonce, counter);
     } else {
-      chacha20_more_than_256(output, plain, len, key, nonce, counter);
-      
+      chacha20_more_than_256(output, plain, len, key, nonce, counter);     
     }
   }
 }.
@@ -109,6 +508,104 @@ proof.
   by inline [tuple] *; sim.
 qed.
 
+equiv eq_column_round :ChaCha20_pref.M.column_round ~ M.column_round : ={k} ==> ={res}.
+proof.
+(* Take few secondes *)
+(*  proc. 
+  conseq (_: Array16.all_eq k{1} k{2}).
+  + by move=> ?????;apply Array16.all_eq_eq.
+  by rewrite /all_eq /=; inline *; wp; skip. 
+qed. *)
+admitted.
+
+equiv eq_diagonal_round :ChaCha20_pref.M.diagonal_round ~ M.diagonal_round : ={k} ==> ={res}.
+proof.
+(* Take few secondes *)
+(*  proc. 
+  conseq (_: Array16.all_eq k{1} k{2}).
+  + by move=> ?????;apply Array16.all_eq_eq.
+  by rewrite /all_eq /=; inline *; wp; skip.
+qed.
+*)
+admitted.
+
+equiv eq_rounds : ChaCha20_pref.M.rounds ~ M.rounds : ={k} ==> ={res}.
+proof.
+  proc; inline ChaCha20_pref.M.round.
+  while (={c, k}); last by auto.
+  by wp; sp; call eq_diagonal_round; call eq_column_round; auto.
+qed.
+
+equiv eq_column_round_x1 : ChaCha20_pref.M.column_round ~M.column_round_x1 : ={k} ==> = {res}.
+proof.
+(* Take few secondes *)
+(*  proc.
+  conseq (_: Array16.all_eq k{1} k{2}).
+  + by move=> ?????;apply Array16.all_eq_eq.
+  by rewrite /all_eq /=; inline *; wp; skip.
+qed.
+*)
+admitted.
+
+equiv eq_diagonal_round_x1 : ChaCha20_pref.M.diagonal_round ~M.diagonal_round_x1 : ={k} ==> = {res}.
+proof.
+(* Take few secondes *)
+(*  proc.
+  conseq (_: Array16.all_eq k{1} k{2}).
+  + by move=> ?????;apply Array16.all_eq_eq.
+  by rewrite /all_eq /=; inline *; wp; skip.
+qed.
+*)
+admitted.
+
+equiv eq_rounds_x1 : ChaCha20_pref.M.rounds ~ M.rounds_x1 : ={k} ==> ={res}.
+proof.
+  proc; inline ChaCha20_pref.M.round.
+  while (={c, k}); last by auto.
+  by wp; sp; call eq_diagonal_round_x1; call eq_column_round_x1; auto.
+qed.
+
+equiv eq_line_x4: M.line_x4 ~ M.line_x4 : ={arg} ==> ={res}.
+proof. by sim. qed.
+
+equiv eq_column_round_x2_aux : M.column_round_x2_aux ~ M.column_round_x2 : 
+ k1_1{1} = k1{2} /\ k1_2{1} = k2{2} ==> ={res}.
+proof.
+  proc => /=.
+  inline [-tuple] M.line_x8 M.column_round.
+  interleave{1} [1:1] [7:1] 6.
+  by do 4! (wp; do 2! call eq_line_x4); wp; skip.
+qed.
+
+equiv eq_rounds_x2 : M.rounds_x2_aux ~ M.rounds_x2 : ={k1_1, k1_2} ==> ={res}.
+proof.
+  proc => /=.
+  inline M.rounds. swap{1} 4 3. swap{1} 4 -2; sp 2 0; wp.
+  transitivity* {1} { c <- 0; 
+                      while (c < 10) {
+                        k <@ M.column_round(k);
+                        k <@ M.diagonal_round(k);
+                        k0 <@ M.column_round(k0);
+                        k0 <@ M.diagonal_round(k0);
+                        c <- c + 1;
+                      }
+                    }.
+  + smt(). + done.
+  + unroll for{1} 4; unroll for{1} 2; unroll for{2} 2.
+    by interleave{1} [1:3] [32:3] 10; sim.
+  while (#post /\ ={c});last by auto.
+  wp; swap{1} 3 -1; conseq />.
+  inline M.diagonal_round M.diagonal_round_x2.
+  interleave{1} [3:1] [8:1] 5.
+  transitivity* {1} { (k, k0) <@ M.column_round_x2_aux(k, k0); 
+                      (k, k0) <@ M.shuffle_state(k, k0); 
+                      (k, k0) <@ M.column_round_x2_aux(k, k0); 
+                      (k, k0) <@ M.reverse_shuffle_state(k, k0); }.
+  + smt (). + done. 
+  + by inline M.column_round_x2_aux M.shuffle_state M.reverse_shuffle_state; sim.
+  sim (_: true); conseq eq_column_round_x2_aux.
+qed.
+
 equiv eq_chacha20_less_than_257 : ChaCha20_avx2_pv.M.chacha20_less_than_257 ~ M.chacha20_less_than_257 :
    ={output, plain, len, key, nonce, counter, Glob.mem} ==> 
    ={Glob.mem}.
@@ -119,1022 +616,289 @@ proof.
   if => //; last first.
   + inline ChaCha20_avx2_pv.M.chacha20_less_than_128; sim.
     swap{1} 7 -2. interleave{1} [6:1] [8:1] 2.  
-    inline [-tuple] M.sum_states_x2 ChaCha20_pref.M.increment_counter M.rounds_x2 ChaCha20_pref.M.rounds; sim.
-    swap{1} 11 3. swap{1} 11 -2.
-    wp; sp 9 2.  
-    transitivity * {1} {
-      c <- 0;
-      while (c < 10) {
-        k <@ ChaCha20_pref.M.round(k);
-        k0 <@ ChaCha20_pref.M.round(k0);
-        c <- c + 1;
-      }
-    }.
+    inline [-tuple] M.sum_states_x2 ChaCha20_pref.M.increment_counter; sim.
+    sp 7 0.  
+    transitivity * {1} { (k_1, k_2) <@ M.rounds_x2_aux(st_10, st_20); }.
     + smt(). + done.
-    + unroll for {1} 4;unroll for {1} 2;unroll for {2} 2.
-      by interleave{1} [1:2] [22:2] 10; sim.
+    + inline M.rounds_x2_aux; wp.
+      by do 2! call eq_rounds; wp; skip.
+    by call eq_rounds_x2; auto.
+  inline{1} ChaCha20_avx2_pv.M.chacha20_between_128_255; sim.
+  swap{1} 7 -2. swap{1} 10 -4. swap{1} 13 -6. 
+  interleave{1} [8:1] [10:1] [12:1] [14:1] 2.
+  inline ChaCha20_pref.M.increment_counter M.copy_state_x4 M.rounds_x4.
+  sp 13 9; conseq />.
+  seq 4 3 : (#post /\ st_10{1} = st_1{2} /\ st_20{1} = st_2{2} /\ 
+                      st_30{1} = st_1{2}.[12 <- st_1{2}.[12] + W32.of_int 2] /\
+                      st_4{1}  = st_2{2}.[12 <- st_2{2}.[12] + W32.of_int 2]).
+  + conseq (_: k_4{1} = k2_2{2} /\ k_3{1} = k2_1{2} /\ k_2{1} = k1_2{2} /\ k_1{1} = k1_1{2}) => //.
+    transitivity * {1} { (k_1, k_2) <@ M.rounds_x2_aux(st_10, st_20);
+                         (k_3, k_4) <@ M.rounds_x2_aux(st_30, st_4); }.
+    + smt(). + done.
+    + inline M.rounds_x2_aux; wp.
+      by do 4! (call eq_rounds; wp); skip.
+    transitivity * {1} { (k_1, k_2) <@ M.rounds_x2(st_10, st_20);
+                         (k_3, k_4) <@ M.rounds_x2(st_30, st_4); }.
+    + smt(). + done.
+    + by wp; do 2!call eq_rounds_x2; auto.
+    inline [-tuple] M.rounds_x2.
+    swap{1} [5..8] 4. swap{1} [5..6] -2; wp; sp 4 0.
+    transitivity* {1} {
+      c <- 0;
+      while(c < 10) {
+       (k1_10, k1_20) <@ M.column_round_x2(k1_10, k1_20);
+       (k1_10, k1_20) <@ M.diagonal_round_x2(k1_10, k1_20);
+       (k1_11, k1_21) <@ M.column_round_x2(k1_11, k1_21);
+       (k1_11, k1_21) <@ M.diagonal_round_x2(k1_11, k1_21);
+       c <- c + 1;
+     } }.
+    + smt(). + done.
+    + unroll for{1} 4; unroll for{1} 2; unroll for{2} 2.
+      by interleave{1} [1:3] [32:3] 10; sim.
     while (#post /\ ={c}); last by auto.
-    inline [-tuple] ChaCha20_pref.M.round M.column_round_x2 M.diagonal_round_x2.
-    by swap{1} [5..6] -2; wp; sim />. 
-  
- 
-
-inline ChaCha20_pref.M.rounds.
- 
-    transitivity * {  
-inline [-tuple] ChaCha20_avx2_pv.M.chacha20_less_than_128 ChaCha20_avx2_pv.M.chacha20_body; sim.
-    inline{1} (2) ChaCha20_pref.M.increment_counter; wp.
-    swap{1} 8 -2. 
-    inline [-tuple] M.sum_states_x2; wp.
-    swap{1} [8..9] 1. swap{1} [9..11] 3. sim.
-    replace * {1} {_ as c1; (_ <@ _; _; _ <@ _) as c2} by 
-                  {c1; 
-                   (k,k0) <@ M.rounds_x2_aux(st0, st1);
-                   st2 <- st1; }.
-    + smt (). + done.
-    + by inline M.rounds_x2_aux; sim.
-    wp; call rounds_x2_aux_rounds_x2.
-    by inline ChaCha20_pref.M.increment_counter; auto.
-  inline{1} ChaCha20_avx2_pv.M.chacha20_between_128_255_1.
-  inline{1} [-tuple] ChaCha20_avx2_pv.M.chacha20_body ChaCha20_avx2_pv.M.chacha20_less_than_128.
-  swap{1} 11 -1. swap{1} [9..10] 10.
-  swap{1} 14 -2. swap{1} [8..12] -2.
-  swap{1} [19..24] 17.
-  swap{1} 23 -2. swap{1} [18..21] -1. swap{1} [16..20] -5.
-  swap{1} 31 -2. swap{1} [27..29] -1. swap{1} [25..28] -9.
-  swap{1} 21 1. swap{1} [22..25] 1. swap{1} [23..29] 1. 
-  inline{2} [-tuple] M.sum_states_x4 M.sum_states_x2; sim.
-  wp.
-  
-
-swap{1} [24..29] 1. swap{1} [25..
-  
-  swap{1} 16 -2.
-  
-
+    wp; swap{1} 3 -1; conseq />.
+    inline M.column_round_x4 M.diagonal_round_x4 M.shuffle_state_x2 M.reverse_shuffle_state_x2
+       M.diagonal_round_x2.
+    by swap{1} [9..11] -3; swap{1} 12 -2; sim.    
+  conseq />; inline M.sum_states_x4; sp; wp.
+  seq 2 1: (k_1{1} = k1_11{2} /\ k_2{1} = k1_21{2} /\ k_3{1} = k2_11{2} /\ k_4{1} = k2_21{2} /\
+                      st_30{1} = st_11{2}.[12 <- st_11{2}.[12] + W32.of_int 2] /\
+                      st_4{1}  = st_21{2}.[12 <- st_21{2}.[12] + W32.of_int 2]).
+  + by inline M.sum_states_x2; sim />.
+  inline M.sum_states_x2 ChaCha20_pref.M.sum_states; wp. sp 2 6.
+  conseq (_: Array16.all_eq k0{1} k0{2}.[12 <- k0{2}.[12] + (of_int 2)%W32] /\ 
+             Array16.all_eq k_3{1} k1{2}.[12 <- k1{2}.[12] + (of_int 2)%W32]).
+  + by move=> |> ???? /Array16.all_eq_eq -> /Array16.all_eq_eq ->.
+  (* FIXME : unroll for 7; unroll for 2. *)
+  unroll for{1} 7; unroll for{1} 2.
+  unroll for{2} 7; unroll for{2} 2.
+  rewrite /Array16.all_eq /=; wp; skip => />.
+  (* FIXME: move=> &2; ring. *)
+  move=> &2; split; ring.
 qed.
 
+op is_incr_count8 (st1: W32.t Array16.t) (st2: W32.t Array16.t Array8.t) = 
+   st2 = Array8.init (fun i => st1.[12 <- st1.[12] + W32.of_int i]).
 
+equiv eq_line_x1_x8 :
+   M.line_x1_8 ~ M.line_x8_v :
+   ={a,b,c,r} /\
+   k{2} = Array8.of_list witness 
+            [k1{1}; k2{1}; k3{1}; k4{1}; k5{1}; k6{1}; k7{1}; k8{1}] ==>
+   res{2} = 
+     Array8.of_list witness 
+      [res{1}.`1; res{1}.`2; res{1}.`3; res{1}.`4; res{1}.`5; res{1}.`6; res{1}.`7; res{1}.`8].
+proof.
+  proc => /=. 
+  conseq (_: Array8.all_eq k{2} 
+             (Array8.of_list witness [k1{1}; k2{1}; k3{1}; k4{1}; k5{1}; k6{1}; k7{1}; k8{1}])).
+  + by move=> *;apply Array8.all_eq_eq.
+  unroll for{2} 2.
+  by do !(wp; call (_:true) => /=; 1: by sim); wp; skip.
+qed.
 
-  inline [-tuple] M.rounds_x2 ChaCha20_pref.M.rounds.
-  
-    
-  inline 
-  
-  interleave{2} [2:1] [4:1] 2.
-  interleave{
-  transitivity{1}
-    {
-      output0 <- output;
-      plain0 <- plain;                             
-      len0 <- len;                               
-      st <- st_1;                                   
-      st0 <- st;                                     
-      st1 <@ ChaCha20_pref.M.increment_counter(st0);
-      k <@ ChaCha20_pref.M.rounds(st0); 
-      k <@ ChaCha20_avx2_pv.M.sum_states(k, st0);
-      k1_10 <- k;
-      st_20 <- st1;    
-      st2 <- st_20;                    
-      k0 <@ ChaCha20_pref.M.rounds(st2);
-      k0 <@ ChaCha20_avx2_pv.M.sum_states(k0, st2);
+equiv eq_line_2_x1_x8 :
+   M.line_2_x1_8 ~ M.line_2_x8_v :
+  ={a0,b0,c0,r0, a1,b1,c1,r1} /\
+   k{2} = Array8.of_list witness 
+            [k1{1}; k2{1}; k3{1}; k4{1}; k5{1}; k6{1}; k7{1}; k8{1}] ==>
+   res{2} = 
+     Array8.of_list witness 
+      [res{1}.`1; res{1}.`2; res{1}.`3; res{1}.`4; res{1}.`5; res{1}.`6; res{1}.`7; res{1}.`8].
+proof.
+  proc => /=. 
+  conseq (_: Array8.all_eq k{2} 
+             (Array8.of_list witness [k1{1}; k2{1}; k3{1}; k4{1}; k5{1}; k6{1}; k7{1}; k8{1}])).
+  + by move=> *;apply Array8.all_eq_eq.
+  unroll for{2} 2.
+  by do !(wp; call (_:true) => /=; 1: by sim); wp; skip.
+qed.
+
+equiv eq_double_quarter_round_x1_x8 :
+   M.double_quarter_round_x1_8 ~ M.double_quarter_round_x8 :
+   ={a0,b0,c0,d0, a1,b1,c1,d1} /\
+   k{2} = Array8.of_list witness 
+            [k1{1}; k2{1}; k3{1}; k4{1}; k5{1}; k6{1}; k7{1}; k8{1}] ==>
+   res{2} = 
+     Array8.of_list witness 
+      [res{1}.`1; res{1}.`2; res{1}.`3; res{1}.`4; res{1}.`5; res{1}.`6; res{1}.`7; res{1}.`8].
+proof.
+  proc => /=.
+  inline M.double_quarter_round_x1.
+  interleave{1} [1:9] [16:9] [31:9] [46:9] [61:9] [76:9] [91:9] [106:9] 1 .
+  interleave{1} [73:1] [79:1] [85:1] [91:1] [97:1] [103:1] [109:1] [115:1] 5.
+  wp.
+  replace * {1} { [1..72]! _ as c; _} by {
+    c;
+    (k, k0, k9, k10, k11, k12, k13, k14) <@ 
+       M.line_x1_8(k, k0, k9, k10, k11, k12, k13, k14, a0, b0, d0, 16);
+    (k, k0, k9, k10, k11, k12, k13, k14) <@
+       M.line_2_x1_8(k, k0, k9, k10, k11, k12, k13, k14, c0, d0, b0, 12, a1, b1, d1, 16); 
+    (k, k0, k9, k10, k11, k12, k13, k14) <@
+       M.line_2_x1_8(k, k0, k9, k10, k11, k12, k13, k14, a0, b0, d0, 8, c1, d1, b1, 12);
+    (k, k0, k9, k10, k11, k12, k13, k14) <@
+       M.line_2_x1_8(k, k0, k9, k10, k11, k12, k13, k14, c0, d0, b0, 7, a1, b1, d1, 8);
+    (k, k0, k9, k10, k11, k12, k13, k14) <@
+       M.line_x1_8(k, k0, k9, k10, k11, k12, k13, k14, c1, d1, b1, 7);
+  }. + smt(). + done.
+  + inline M.line_x1_8 M.line_2_x1_8.
+    by do !(wp;call (_:true) => /=; 1:by sim);wp; skip => />.
+  call eq_line_x1_x8; do 3! call eq_line_2_x1_x8; call eq_line_x1_x8; wp; skip => />.
+qed.
+
+equiv eq_body_x8 : ChaCha20_avx2_pv.M.body_x8 ~ M.body_x8 : 
+   is_incr_count8 st_1{1} st{2} ==>
+   is_incr_count8 res{1}.`1 res{2}.`2 /\
+   res{2}.`1 = Array8.of_list witness [res{1}.`2; res{1}.`3; res{1}.`4; res{1}.`5;
+                                       res{1}.`6; res{1}.`7; res{1}.`8; res{1}.`9].
+proof.
+  proc => /=.
+  swap{1} 3 -2, {1} 6 -4, {1} 9 -6, {1} 12 -8, {1} 15 -10, {1} 18 -12, {1} 21 -14. 
+  interleave{1} [8:1] [10:1] [12:1] [14:1] [16:1] [18:1] [20:1] [22:1] 2.
+  seq 7 0 : (is_incr_count8 st_1{1} st{2} /\
+             st{2} = Array8.of_list witness [st_1{1}; st_2{1}; st_3{1}; st_4{1}; 
+                                             st_5{1}; st_6{1}; st_7{1}; st_8{1} ]).
+  + conseq (_:Array8.all_eq st{2} (Array8.of_list witness [st_1{1}; st_2{1}; st_3{1}; st_4{1}; 
+                                                           st_5{1}; st_6{1}; st_7{1}; st_8{1} ])).
+    + by move=> |> *;apply Array8.all_eq_eq.
+    inline ChaCha20_pref.M.increment_counter;wp; skip; rewrite /Array8.all_eq /= /is_incr_count8.
+    by move=> &1 &2 -> /=; rewrite set_notmod.
+  seq 8 1 : (#pre /\ k{2} = Array8.of_list witness [k_1{1}; k_2{1}; k_3{1}; k_4{1}; 
+                                                    k_5{1}; k_6{1}; k_7{1}; k_8{1} ]).
+  + conseq |>.
+    transitivity*{1} {
+      k_1 <@ M.rounds_x1(st_1);
+      k_2 <@ M.rounds_x1(st_2);
+      k_3 <@ M.rounds_x1(st_3);
+      k_4 <@ M.rounds_x1(st_4);
+      k_5 <@ M.rounds_x1(st_5);
+      k_6 <@ M.rounds_x1(st_6);
+      k_7 <@ M.rounds_x1(st_7);
+      k_8 <@ M.rounds_x1(st_8);
+    }. + smt(). + done.
+    by do 8! call eq_rounds_x1; skip => />.
+    inline M.rounds_x1.
+    transitivity*{1} {
+      (k_1, k_2, k_3, k_4, k_5, k_6, k_7, k_8) <- 
+        (st_1, st_2, st_3, st_4, st_5, st_6, st_7, st_8);
+      c <- 0;
+      while(c < 10) {
+        k_1 <@ M.column_round_x1(k_1);  
+        k_1 <@ M.diagonal_round_x1(k_1);  
+        k_2 <@ M.column_round_x1(k_2);  
+        k_2 <@ M.diagonal_round_x1(k_2);  
+        k_3 <@ M.column_round_x1(k_3);  
+        k_3 <@ M.diagonal_round_x1(k_3);  
+        k_4 <@ M.column_round_x1(k_4);   
+        k_4 <@ M.diagonal_round_x1(k_4);   
+        k_5 <@ M.column_round_x1(k_5);   
+        k_5 <@ M.diagonal_round_x1(k_5);   
+        k_6 <@ M.column_round_x1(k_6);   
+        k_6 <@ M.diagonal_round_x1(k_6);   
+        k_7 <@ M.column_round_x1(k_7);   
+        k_7 <@ M.diagonal_round_x1(k_7);   
+        k_8 <@ M.column_round_x1(k_8);
+        k_8 <@ M.diagonal_round_x1(k_8);
+        c <- c + 1;
+      }
+    }. + smt(). + done.
+    + interleave{1} [1:1] [5:1] [9:1] [13:1] [17:1] [21:1] [25:1] [29:1] 1.
+      interleave{1} [9:2] [12:2] [15:2] [18:2] [21:2] [24:2] [27:2] [30:2] 1.
+      (* FIXME unroll for{1} 10 12 14 16 18 20 22 24. *)
+      wp; unroll for{1} 24; unroll for{1} 22; unroll for{1} 20; unroll for{1} 18; unroll for{1} 16;
+        unroll for{1} 14; unroll for{1} 12; unroll for{1} 10.
+      interleave{1} [9:3] [40:3] [71:3] [102:3] [133:3] [164:3] [195:3] [226:3] 10.
+      by unroll for{2} 3; sim.
+    inline M.rounds_x8;wp.
+    while (={c} /\ #post);last by auto.
+    wp; conseq />.
+    interleave {1} [1:1] [3:1] [5:1] [7:1] [9:1] [11:1] [13:1] [15:1] 1.
+    seq 8 1: (#post).
+    + inline M.column_round_x8 M.column_round_x1.
+      interleave{1} [1:1] [5:1] [9:1] [13:1] [17:1] [21:1] [25:1] [29:1] 1.
+      interleave{1} [9:1] [12:1] [15:1] [18:1] [21:1] [24:1] [27:1] [30:1] 1.
+      interleave{1} [17:1] [19:1] [21:1] [23:1] [25:1] [27:1] [29:1] [31:1] 1.
+      wp. sp.
+      transitivity*{1}{
+        (k7,k8,k9,k10,k11,k12,k13,k14) <@ M.double_quarter_round_x1_8
+          (k7,k8,k9,k10,k11,k12,k13,k14, 0, 4, 8, 12, 2, 6, 10, 14);
+        (k7,k8,k9,k10,k11,k12,k13,k14) <@ M.double_quarter_round_x1_8
+          (k7,k8,k9,k10,k11,k12,k13,k14, 1, 5, 9, 13, 3, 7, 11, 15);
+      }. + smt(). + done. 
+      + inline M.double_quarter_round_x1_8.
+        by do !(wp; call (_:true) => /=; 1: by sim); wp; skip => />.
+      by do 2! call eq_double_quarter_round_x1_x8; skip.
+    inline M.diagonal_round_x8 M.diagonal_round_x1.
+    interleave{1} [1:1] [5:1] [9:1] [13:1] [17:1] [21:1] [25:1] [29:1] 1.
+    interleave{1} [9:1] [12:1] [15:1] [18:1] [21:1] [24:1] [27:1] [30:1] 1.
+    interleave{1} [17:1] [19:1] [21:1] [23:1] [25:1] [27:1] [29:1] [31:1] 1.
+    wp. sp.
+    transitivity*{1}{
+      (k7,k8,k9,k10,k11,k12,k13,k14) <@ M.double_quarter_round_x1_8
+        (k7,k8,k9,k10,k11,k12,k13,k14, 1, 6, 11, 12, 0, 5, 10, 15);
+      (k7,k8,k9,k10,k11,k12,k13,k14) <@ M.double_quarter_round_x1_8
+        (k7,k8,k9,k10,k11,k12,k13,k14, 2, 7, 8, 13, 3, 4, 9, 14);
+    }. + smt(). + done. 
+    + inline M.double_quarter_round_x1_8.
+      by do !(wp; call (_:true) => /=; 1: by sim); wp; skip => />.
+    by do 2! call eq_double_quarter_round_x1_x8; skip.
+  seq 8 1 : (#pre).  
+  + conseq />; inline M.sum_states_x8.      
+    unroll for{2} 4.
+    do !(wp; call (_:true) =>/=;1: by sim); wp; skip => />.
+    by move=> &1 ? 8?; apply Array8.all_eq_eq.
+  conseq />; inline *; rewrite /is_incr_count8.
+  unroll for{2} 3; wp; skip=> &1 &2 [#] -> /Array8.ext_eq_all /> ?.
+  by apply Array8.all_eq_eq; rewrite /Array8.all_eq /=.
+qed.
+
+equiv eq_chacha20_more_than_256 : ChaCha20_avx2_pv.M.chacha20_more_than_256 ~ M.chacha20_more_than_256 :
+   ={output, plain, len, key, nonce, counter, Glob.mem} ==> 
+   ={Glob.mem}.
+proof.
+  proc => /=.
+  seq 1 1 : (={output, plain, len, Glob.mem} /\ is_incr_count8 st_1{1} st{2}).
+  + conseq />; inline M.init_x8; wp.
+    call (_: ={Glob.mem}); 1: by sim.
+    wp; skip => />.
+    move=> &2 st; rewrite /is_incr_count8.
+    by apply Array8.all_eq_eq => />; rewrite set_notmod.
+  transitivity* {2} {
+    while (W32.of_int 512 \ule len) {                          
+      (k,st) <@ M.body_x8(st);
+      (output, plain, len) <@ ChaCha20_avx2_pv.M.store_x8(output, plain, len, 
+                                                          k.[0], k.[1], k.[2], k.[3], 
+                                                          k.[4], k.[5], k.[6], k.[7]);
     }
-    (={output, plain, len, st_1, Glob.mem} ==> ={k0, k1_10, len0, plain0, output0, Glob.mem})
-  
-    ((={output, plain, len, key, nonce, counter, Glob.mem} /\ ={st_1} /\ st_2{2} = st_1{1}.[12 <- st_1{1}.[12] + W32.one]) /\
-     ! ((of_int 128)%W32 \ult len{1}) ==>
-     k0{1} = k2{2} /\
-     k1_10{1} = k1{2} /\ len0{1} = len{2} /\ plain0{1} = plain{2} /\ output0{1} = output{2} /\ ={Glob.mem}) => //.
-   + smt().  
-   + by sim.
-   swap{1} [8 .. 9] 3; sim.
-   swap{1} [8..9] -1.
-   seq 8 0 : (#{/~k0{1}}{ ~ k{1}}post).
-   + by inline *;auto.
-   inline M.rounds_x2.
-   inline ChaCha20_pref.M.rounds.
-   inline M.column_round_x2 M.diagonal_round_x2.
-   sp; wp.
-   transitivity{2} {
-      while (c < 10) {                                
-         k1_12 <@ ChaCha20_pref.M.column_round(k1_11);  
-         k1_22 <@ ChaCha20_pref.M.column_round(k1_21);  
-         k1_11 <@ ChaCha20_pref.M.diagonal_round(k1_12);
-         k1_21 <@ ChaCha20_pref.M.diagonal_round(k1_22);
-         c <- c + 1;                                    
-       }                                               
-       (k1_1, k1_2) <- (k1_11, k1_21);
-     }
-   (k1_11{2} = st_1{2} /\
-  k1_21{2} = st_2{2} /\
-  c{2} = 0 /\
-  k1{1} = st0{1} /\
-  c{1} = W32.zero /\
-  st2{1} = st_2{2} /\
-  st0{1} = st_1{2} /\ len0{1} = len{2} /\ plain0{1} = plain{2} /\ output0{1} = output{2} /\ ={Glob.mem} ==>
+    if (W32.zero \ult len) {   
+      (k,st) <@ M.body_x8(st);                                  
+      ChaCha20_avx2_pv.M.store_x8_last(output, plain, len, k.[0], k.[1], k.[2], k.[3], 
+                                                     k.[4], k.[5], k.[6], k.[7]);
+    }
+  }; [1:smt () |2: done]; last first.
+  + seq 1 1 : (#pre).
+    + while (#pre); last by auto.
+      inline [-tuple] M.body_x8. 
+      by swap{1} 4 1, {1}[5..6] 1, {1} [6..8] 1; sim.
+    if => //.
+    by inline [-tuple] M.increment_counter_x8 M.body_x8; unroll for{1} 6; sim.
+  seq 1 1 : (#pre).
+  + while (#pre); last by auto.
+    call (_: ={Glob.mem}) => /=; 1:sim. 
+    by call eq_body_x8; skip;rewrite /is_incr_count8 => |> &2 _ ??? ->.
+  if => //.
+  call (_: ={Glob.mem}) => /=; 1:sim. 
+  by call eq_body_x8; skip;rewrite /is_incr_count8 => |> &2 _ ??? ->.
+qed.
 
-    k2{1} = k1_21{2} /\
-  st2{1} = st_2{2} /\
-  k{1} = k1_11{2} /\
-  st0{1} = st_1{2} /\ len0{1} = len{2} /\ plain0{1} = plain{2} /\ output0{1} = output{2} /\ ={Glob.mem})
-  (={c,k1_11, k1_12, Glob.mem, st_1, st_2, output, plain, len} ==> ={k1_11, k1_21, st_1, st_2, Glob.mem,output, plain, len}) => //. 
-  + smt().
-  + admit.
-  while (#pre).
-
- 
-deadcode.
-constprop.
-
-
- st0{1} = st_1{2} /\ st2{1} = st_2{2} /\ 
-
-len0{1} = len{2} /\ plain0{1} = plain{2} /\ output0{1} = output{2} /\ ={Glob.mem}
-   sim.
-  splittuple 
-
-
-
-
-
-  swap{1} 6 -3.
 equiv eq_chacha20_avx2 : ChaCha20_avx2_pv.M.chacha20_avx2 ~ M.chacha20_avx2 :
    ={output, plain, len, key, nonce, counter, Glob.mem} ==> 
    ={Glob.mem}.
 proof.
   proc => /=.
-  if => //.
-
-  
-
-module M = {
-  proc shuffle_state_1 (st:W32.t Array16.t) : W32.t Array16.t = {
-    var st':W32.t Array16.t;
-    st'.[0]  <- st.[0];
-    st'.[1]  <- st.[1];
-    st'.[2]  <- st.[2];
-    st'.[3]  <- st.[3];
-             
-    st'.[4]  <- st.[5];
-    st'.[5]  <- st.[6];
-    st'.[6]  <- st.[7];
-    st'.[7]  <- st.[4];
-
-    st'.[8]  <- st.[10];
-    st'.[9]  <- st.[11];
-    st'.[10] <- st.[8];
-    st'.[11] <- st.[9];
-
-    st'.[12] <- st.[15];
-    st'.[13] <- st.[12];
-    st'.[14] <- st.[13];
-    st'.[15] <- st.[14];
-    return st';
-  }
-
- proc reverse_shuffle_state_1 (st':W32.t Array16.t) : W32.t Array16.t = {
-    var st:W32.t Array16.t;
-    st.[0]  <- st'.[0];
-    st.[1]  <- st'.[1];
-    st.[2]  <- st'.[2];
-    st.[3]  <- st'.[3];
-                       
-    st.[5]  <- st'.[4];
-    st.[6]  <- st'.[5];
-    st.[7]  <- st'.[6];
-    st.[4]  <- st'.[7];
-                       
-    st.[10] <- st'.[8];
-    st.[11] <- st'.[9];
-    st.[8]  <- st'.[10];
-    st.[9]  <- st'.[11];
-                       
-    st.[15] <- st'.[12];
-    st.[12] <- st'.[13];
-    st.[13] <- st'.[14];
-    st.[14] <- st'.[15];
-    return st;
-  }
-
- proc rotate_1(k:W32.t Array16.t, i r : int) :  W32.t Array16.t = {
-   k.[i + 0] <- W32.rol k.[i + 0] r;
-   k.[i + 1] <- W32.rol k.[i + 1] r;
-   k.[i + 2] <- W32.rol k.[i + 2] r;
-   k.[i + 3] <- W32.rol k.[i + 3] r;
-   return k;
- }
-
- proc line_1 (k:W32.t Array16.t, a b c r : int) : W32.t Array16.t = {
-   var i, a4, b4, c4 : int;
-   i <- 0;
-  
-   k.[a + 0] <-  k.[a + 0] + k.[b + 0];
-   k.[a + 1] <-  k.[a + 1] + k.[b + 1];
-   k.[a + 2] <-  k.[a + 2] + k.[b + 2];
-   k.[a + 3] <-  k.[a + 3] + k.[b + 3];
-
-   k.[c + 0] <-  k.[c + 0] `^` k.[a + 0];
-   k.[c + 1] <-  k.[c + 1] `^` k.[a + 1];
-   k.[c + 2] <-  k.[c + 2] `^` k.[a + 2];
-   k.[c + 3] <-  k.[c + 3] `^` k.[a + 3];
-
-   k <@ rotate_1(k, c, r);
-   return k;   
- }
-
- proc column_round_1 (k:W32.t Array16.t) : W32.t Array16.t = {
-   k <@ line_1(k, 0, 4, 12, 16);
-   k <@ line_1(k, 8, 12, 4, 12);
-   k <@ line_1(k, 0, 4, 12,  8);
-   k <@ line_1(k, 8, 12, 4,  7);
-  return k;
- }
-
- proc diagonal_round_1(k:W32.t Array16.t) : W32.t Array16.t = {
-   var k1, k2, k3 : W32.t Array16.t; 
-   k1 <@ shuffle_state_1(k);
-   k2 <@ column_round_1(k1);
-   k3 <@ reverse_shuffle_state_1(k2);
-   return k3;
- }
-
- proc round_1 (k:W32.t Array16.t) : W32.t Array16.t = {
-   var k1, k2 : W32.t Array16.t; 
-   k1 <@ column_round_1 (k);
-   k2 <@ diagonal_round_1 (k1);
-   return k2;
- }
-
- proc rounds_1 (k:W32.t Array16.t) : W32.t Array16.t = {
-   var c : int;
-   while (c < 20) {
-     k <@ round_1(k);
-     c <- c + 1;
-   }
-   return k;
- }
-   
- proc shuffle_state_2 (st1, st2:W32.t Array16.t) : W32.t Array16.t * W32.t Array16.t = {
-   st1 <@ shuffle_state_1(st1);
-   st2 <@ shuffle_state_1(st2);
-   return (st1, st2);
- }
-
- proc reverse_shuffle_state_2 (st1, st2:W32.t Array16.t) : W32.t Array16.t * W32.t Array16.t = {
-   st1 <@ reverse_shuffle_state_1(st1);
-   st2 <@ reverse_shuffle_state_1(st2);
-   return (st1, st2);
- }
-
-
- proc rotate_2 (k1 k2:W32.t Array16.t, i r : int) :  W32.t Array16.t * W32.t Array16.t = {
-   k1 <@ rotate_1(k1, i, r);
-   k2 <@ rotate_1(k2, i, r);
-   return (k1, k2);
- }
-
- proc line_2 (k1 k2:W32.t Array16.t, a b c r : int) :  W32.t Array16.t * W32.t Array16.t = {
-   k1 <@ line_1(k1, a, b, c, r);
-   k2 <@ line_1(k2, a, b, c, r);
-   return (k1, k2);
- }
-
- proc column_round_2 (k1 k2:W32.t Array16.t) : W32.t Array16.t  * W32.t Array16.t = {
-   (k1, k2) <@ line_2(k1, k2, 0, 4, 12, 16);
-   (k1, k2) <@ line_2(k1, k2, 8, 12, 4, 12);
-   (k1, k2) <@ line_2(k1, k2, 0, 4, 12,  8);
-   (k1, k2) <@ line_2(k1, k2, 8, 12, 4,  7);
-  return (k1, k2);
- }
-
- proc diagonal_round_2(k1, k2:W32.t Array16.t) : W32.t Array16.t * W32.t Array16.t = {
-   var k1_1, k1_2, k2_1, k2_2, k1_3, k2_3 : W32.t Array16.t; 
-   (k1_1, k2_2) <@ shuffle_state_2(k1, k2);
-   (k1_2, k2_2) <@ column_round_2(k1_1, k2_1);
-   (k1_3, k2_3) <@ reverse_shuffle_state_2(k2_1, k2_2);
-   return (k1_3, k2_3);
- }
-
- proc round_2 (k1 k2:W32.t Array16.t) : W32.t Array16.t * W32.t Array16.t = {
-   var k1_1, k1_2, k2_1, k2_2 : W32.t Array16.t; 
-   (k1_1, k2_1) <@ column_round_2 (k1, k2);
-   (k1_2, k2_2) <@ diagonal_round_2 (k1_1, k2_1);
-   return (k1_2, k2_2);
- }
-
- proc rounds_1_2 (k1 k2:W32.t Array16.t) : W32.t Array16.t * W32.t Array16.t = {
-   var c : int;
-   k1 <@ rounds_1(k1);
-   k2 <@ rounds_1(k2);
-   return (k1, k2);
- }
-
- proc rounds_2 (k1 k2:W32.t Array16.t) : W32.t Array16.t * W32.t Array16.t = {
-   var c : int;
-   while (c < 20) {
-     (k1, k2) <@ round_2(k1, k2);
-     c <- c + 1;
-   }
-   return (k1, k2);
- }
-
- proc chacha20_less_than_128 (output:W64.t, plain:W64.t, len:W32.t, st1 st2 : W32.t Array16.t) : unit = {
-   (k1,k2) <@ rounds_2 
-}.
-
-
-
-proc chacha20_less_than_128 (output:W64.t, plain:W64.t, len:W32.t, st : W32.t Array16.t) : unit = {
-     var k1_1:W32.t Array16.t;
-     var st_2:W32.t Array16.t;
-     var k1_2:W32.t Array16.t;
-     var st_3:W32.t Array16.t;
-     (k1_1, st_2) <@ chacha20_body (st);
-     (k1_2, st_3) <@ chacha20_body (st_2);
-     store_x2_last (output, plain, len, k1_1, k1_2);
-  }
-
-
-
-
-
-
-(* proc round_x2(k1:W32.t Array16.t, k2:W32.t Array16.t) : W32.t Array16.t *  W32.t Array16.t = {
-   (k1, k2) = column_round_x2  (k1, k2)
-   (k1, k2) = diagonal_round_x2(k1, k2)
-   return (k1, k2)
- proc rounds_x2 *)
-}.
-
-(*
-hoare test k0 : M.id : k = k0 ==> Array16.all_eq k0 res.
-proof.
-  rewrite /Array16.all_eq /=.
-  proc. 
-  inline *; wp; skip => &hr heq /=.
-  rewrite heq //=.
-qed.
-*)
-
-equiv eq_column_round : ChaCha20_pref.M.column_round ~ M.column_round : ={k} ==> ={res}.
-proof.
-  conseq (_: Array16.all_eq res{1} res{2}).
-  + move=> &1 &2 ???; apply Array16.all_eq_eq.
-  rewrite /Array16.all_eq /=.
-  proc; inline *; wp; skip.
-  move=> &1 &2 heq; cbv delta; rewrite heq //=.
+  if => //; 1: by call eq_chacha20_less_than_257; auto.
+  by call eq_chacha20_more_than_256;auto.  
 qed.
 
-equiv diagonal_round_pref_shuffle1 : ChaCha20_pref.M.diagonal_round ~ M.diagonal_round :
-  ={k} ==> ={res}.
-proof.
-  conseq (_: Array16.all_eq res{1} res{2}).
-  + move=> &1 &2 ???; apply Array16.all_eq_eq.
-  rewrite /Array16.all_eq /=.
-  proc; inline *; wp; skip.
-  move => &1 &2 heq /=; rewrite heq //=.
-qed. 
-admitted.
-
-
-rewrite /Array16.all
-
   
-
-abbrev bswap = W128.of_int 5233100606242806050955395731361295.
-
-
-module M = {
-  proc init (key:W64.t, nonce:W64.t, counter:W32.t) : W32.t Array16.t = {
-    var aux: int;
-    
-    var st:W32.t Array16.t;
-    var i:int;
-    st <- witness;
-    st.[0] <- (W32.of_int 1634760805);
-    st.[1] <- (W32.of_int 857760878);
-    st.[2] <- (W32.of_int 2036477234);
-    st.[3] <- (W32.of_int 1797285236);
-    i <- 0;
-    while (i < 8) {
-      st.[(4 + i)] <- (loadW32 Glob.mem (key + (W64.of_int (4 * i))));
-      i <- i + 1;
-    }
-    st.[12] <- counter;
-    i <- 0;
-    while (i < 3) {
-      st.[(13 + i)] <- (loadW32 Glob.mem (nonce + (W64.of_int (4 * i))));
-      i <- i + 1;
-    }
-    return (st);
-  }
-  
-  proc init_x2 (key:W64.t, nonce:W64.t, counter:W32.t) : W32.t Array16.t *
-                                                         W32.t Array16.t = {
-    
-    var st_1:W32.t Array16.t;
-    var st_2:W32.t Array16.t;
-    st_1 <- witness;
-    st_2 <- witness;
-    st_1 <@ init (key, nonce, counter);
-    counter <- (counter + (W32.of_int 1));
-    st_2 <@ init (key, nonce, counter);
-    return (st_1, st_2);
-  }
-  
-  proc init_x8 (key:W64.t, nonce:W64.t, counter:W32.t) : W32.t Array16.t *
-                                                         W32.t Array16.t *
-                                                         W32.t Array16.t *
-                                                         W32.t Array16.t *
-                                                         W32.t Array16.t *
-                                                         W32.t Array16.t *
-                                                         W32.t Array16.t *
-                                                         W32.t Array16.t = {
-    
-    var st_1:W32.t Array16.t;
-    var st_2:W32.t Array16.t;
-    var st_3:W32.t Array16.t;
-    var st_4:W32.t Array16.t;
-    var st_5:W32.t Array16.t;
-    var st_6:W32.t Array16.t;
-    var st_7:W32.t Array16.t;
-    var st_8:W32.t Array16.t;
-    st_1 <- witness;
-    st_2 <- witness;
-    st_3 <- witness;
-    st_4 <- witness;
-    st_5 <- witness;
-    st_6 <- witness;
-    st_7 <- witness;
-    st_8 <- witness;
-    st_1 <@ init (key, nonce, counter);
-    counter <- (counter + (W32.of_int 1));
-    st_2 <@ init (key, nonce, counter);
-    counter <- (counter + (W32.of_int 1));
-    st_3 <@ init (key, nonce, counter);
-    counter <- (counter + (W32.of_int 1));
-    st_4 <@ init (key, nonce, counter);
-    counter <- (counter + (W32.of_int 1));
-    st_5 <@ init (key, nonce, counter);
-    counter <- (counter + (W32.of_int 1));
-    st_6 <@ init (key, nonce, counter);
-    counter <- (counter + (W32.of_int 1));
-    st_7 <@ init (key, nonce, counter);
-    counter <- (counter + (W32.of_int 1));
-    st_8 <@ init (key, nonce, counter);
-    return (st_1, st_2, st_3, st_4, st_5, st_6, st_7, st_8);
-  }
-  
-  proc copy_state (st:W32.t Array16.t) : W32.t Array16.t = {
-    
-    var k:W32.t Array16.t;
-    k <- witness;
-    k <- st;
-    return (k);
-  }
-  
-  proc copy_state_x2 (st_1:W32.t Array16.t, st_2:W32.t Array16.t) : W32.t Array16.t *
-                                                                    W32.t Array16.t = {
-    
-    var k_1:W32.t Array16.t;
-    var k_2:W32.t Array16.t;
-    k_1 <- witness;
-    k_2 <- witness;
-    k_1 <@ copy_state (st_1);
-    k_2 <@ copy_state (st_2);
-    return (k_1, k_2);
-  }
-  
-  proc copy_state_x4 (st_1:W32.t Array16.t, st_2:W32.t Array16.t) : W32.t Array16.t *
-                                                                    W32.t Array16.t *
-                                                                    W32.t Array16.t *
-                                                                    W32.t Array16.t = {
-    
-    var k_1:W32.t Array16.t;
-    var k_2:W32.t Array16.t;
-    var k_3:W32.t Array16.t;
-    var k_4:W32.t Array16.t;
-    k_1 <- witness;
-    k_2 <- witness;
-    k_3 <- witness;
-    k_4 <- witness;
-    k_1 <@ copy_state (st_1);
-    k_2 <@ copy_state (st_2);
-    k_3 <@ copy_state (st_1);
-    k_4 <@ copy_state (st_2);
-    k_3.[12] <- (k_3.[12] + (W32.of_int 2));
-    k_4.[12] <- (k_4.[12] + (W32.of_int 2));
-    return (k_1, k_2, k_3, k_4);
-  }
-  
-  proc copy_state_x8 (st_1:W32.t Array16.t, st_2:W32.t Array16.t,
-                      st_3:W32.t Array16.t, st_4:W32.t Array16.t,
-                      st_5:W32.t Array16.t, st_6:W32.t Array16.t,
-                      st_7:W32.t Array16.t, st_8:W32.t Array16.t) : W32.t Array16.t *
-                                                                    W32.t Array16.t *
-                                                                    W32.t Array16.t *
-                                                                    W32.t Array16.t *
-                                                                    W32.t Array16.t *
-                                                                    W32.t Array16.t *
-                                                                    W32.t Array16.t *
-                                                                    W32.t Array16.t = {
-    
-    var k_1:W32.t Array16.t;
-    var k_2:W32.t Array16.t;
-    var k_3:W32.t Array16.t;
-    var k_4:W32.t Array16.t;
-    var k_5:W32.t Array16.t;
-    var k_6:W32.t Array16.t;
-    var k_7:W32.t Array16.t;
-    var k_8:W32.t Array16.t;
-    k_1 <- witness;
-    k_2 <- witness;
-    k_3 <- witness;
-    k_4 <- witness;
-    k_5 <- witness;
-    k_6 <- witness;
-    k_7 <- witness;
-    k_8 <- witness;
-    k_1 <@ copy_state (st_1);
-    k_2 <@ copy_state (st_2);
-    k_3 <@ copy_state (st_3);
-    k_4 <@ copy_state (st_4);
-    k_5 <@ copy_state (st_5);
-    k_6 <@ copy_state (st_6);
-    k_7 <@ copy_state (st_7);
-    k_8 <@ copy_state (st_8);
-    return (k_1, k_2, k_3, k_4, k_5, k_6, k_7, k_8);
-  }
-  
-  proc sum_states (k:W32.t Array16.t, st:W32.t Array16.t) : W32.t Array16.t = {
-    var aux: int;
-    
-    var i:int;
-    
-    i <- 0;
-    while (i < 16) {
-      k.[i] <- (k.[i] + st.[i]);
-      i <- i + 1;
-    }
-    return (k);
-  }
-  
-  proc sum_states_x2 (k_1:W32.t Array16.t, k_2:W32.t Array16.t,
-                      st_1:W32.t Array16.t, st_2:W32.t Array16.t) : W32.t Array16.t *
-                                                                    W32.t Array16.t = {
-    
-    
-    
-    k_1 <@ sum_states (k_1, st_1);
-    k_2 <@ sum_states (k_2, st_2);
-    return (k_1, k_2);
-  }
-  
-  proc sum_states_x4 (k1_1:W32.t Array16.t, k1_2:W32.t Array16.t,
-                      k2_1:W32.t Array16.t, k2_2:W32.t Array16.t,
-                      st_1:W32.t Array16.t, st_2:W32.t Array16.t) : W32.t Array16.t *
-                                                                    W32.t Array16.t *
-                                                                    W32.t Array16.t *
-                                                                    W32.t Array16.t = {
-    
-    
-    
-    (k1_1, k1_2) <@ sum_states_x2 (k1_1, k1_2, st_1, st_2);
-    (k2_1, k2_2) <@ sum_states_x2 (k2_1, k2_2, st_1, st_2);
-    k2_1.[12] <- (k2_1.[12] + (W32.of_int 2));
-    k2_2.[12] <- (k2_2.[12] + (W32.of_int 2));
-    return (k1_1, k1_2, k2_1, k2_2);
-  }
-  
-  proc sum_states_x8 (k_1:W32.t Array16.t, k_2:W32.t Array16.t,
-                      k_3:W32.t Array16.t, k_4:W32.t Array16.t,
-                      k_5:W32.t Array16.t, k_6:W32.t Array16.t,
-                      k_7:W32.t Array16.t, k_8:W32.t Array16.t,
-                      st_1:W32.t Array16.t, st_2:W32.t Array16.t,
-                      st_3:W32.t Array16.t, st_4:W32.t Array16.t,
-                      st_5:W32.t Array16.t, st_6:W32.t Array16.t,
-                      st_7:W32.t Array16.t, st_8:W32.t Array16.t) : W32.t Array16.t *
-                                                                    W32.t Array16.t *
-                                                                    W32.t Array16.t *
-                                                                    W32.t Array16.t *
-                                                                    W32.t Array16.t *
-                                                                    W32.t Array16.t *
-                                                                    W32.t Array16.t *
-                                                                    W32.t Array16.t = {
-    
-    
-    
-    k_1 <@ sum_states (k_1, st_1);
-    k_2 <@ sum_states (k_2, st_2);
-    k_3 <@ sum_states (k_3, st_3);
-    k_4 <@ sum_states (k_4, st_4);
-    k_5 <@ sum_states (k_5, st_5);
-    k_6 <@ sum_states (k_6, st_6);
-    k_7 <@ sum_states (k_7, st_7);
-    k_8 <@ sum_states (k_8, st_8);
-    return (k_1, k_2, k_3, k_4, k_5, k_6, k_7, k_8);
-  }
-  
-  proc update_ptr (output:W64.t, plain:W64.t, len:W32.t, n:int) : W64.t *
-                                                                  W64.t *
-                                                                  W32.t = {
-    
-    
-    
-    output <- (output + (W64.of_int n));
-    plain <- (plain + (W64.of_int n));
-    len <- (len - (W32.of_int n));
-    return (output, plain, len);
-  }
-  
-  proc store (output:W64.t, plain:W64.t, len:W32.t, k:W32.t Array16.t) : 
-  W64.t * W64.t * W32.t = {
-    var aux: int;
-    
-    var i:int;
-    
-    i <- 0;
-    while (i < 16) {
-      k.[i] <- (k.[i] `^` (loadW32 Glob.mem (plain + (W64.of_int (4 * i)))));
-      Glob.mem <- storeW32 Glob.mem (output + (W64.of_int (4 * i))) k.[i];
-      i <- i + 1;
-    }
-    (output, plain, len) <@ update_ptr (output, plain, len, 64);
-    return (output, plain, len);
-  }
-  
-  proc store_last (output:W64.t, plain:W64.t, len:W32.t, k:W32.t Array16.t) : unit = {
-    
-    var s_k:W32.t Array16.t;
-    var j:W64.t;
-    var pi:W8.t;
-    s_k <- witness;
-    s_k <- k;
-    j <- (W64.of_int 0);
-    
-    while (((truncateu32 j) \ult len)) {
-      pi <- (loadW8 Glob.mem (plain + j));
-      pi <-
-      (pi `^` (get8 (WArray64.init32 (fun i => s_k.[i])) (W64.to_uint j)));
-      Glob.mem <- storeW8 Glob.mem (output + j) pi;
-      j <- (j + (W64.of_int 1));
-    }
-    return ();
-  }
-  
-  proc store_x2 (output:W64.t, plain:W64.t, len:W32.t, k_1:W32.t Array16.t,
-                 k_2:W32.t Array16.t) : W64.t * W64.t * W32.t = {
-    
-    
-    
-    (output, plain, len) <@ store (output, plain, len, k_1);
-    (output, plain, len) <@ store (output, plain, len, k_2);
-    return (output, plain, len);
-  }
-  
-  proc store_x2_last (output:W64.t, plain:W64.t, len:W32.t,
-                      k_1:W32.t Array16.t, k_2:W32.t Array16.t) : unit = {
-    
-    var r:W32.t Array16.t;
-    r <- witness;
-    r <- k_1;
-    if (((W32.of_int 64) \ule len)) {
-      (output, plain, len) <@ store (output, plain, len, r);
-      r <- k_2;
-    } else {
-      
-    }
-    store_last (output, plain, len, r);
-    return ();
-  }
-  
-  proc store_x4 (output:W64.t, plain:W64.t, len:W32.t, k_1:W32.t Array16.t,
-                 k_2:W32.t Array16.t, k_3:W32.t Array16.t,
-                 k_4:W32.t Array16.t) : W64.t * W64.t * W32.t = {
-    
-    
-    
-    (output, plain, len) <@ store (output, plain, len, k_1);
-    (output, plain, len) <@ store (output, plain, len, k_2);
-    (output, plain, len) <@ store (output, plain, len, k_3);
-    (output, plain, len) <@ store (output, plain, len, k_4);
-    return (output, plain, len);
-  }
-  
-  proc store_x4_last (output:W64.t, plain:W64.t, len:W32.t,
-                      k_1:W32.t Array16.t, k_2:W32.t Array16.t,
-                      k_3:W32.t Array16.t, k_4:W32.t Array16.t) : unit = {
-    
-    var r_1:W32.t Array16.t;
-    var r_2:W32.t Array16.t;
-    r_1 <- witness;
-    r_2 <- witness;
-    r_1 <- k_1;
-    r_2 <- k_2;
-    if (((W32.of_int 128) \ule len)) {
-      (output, plain, len) <@ store_x2 (output, plain, len, r_1, r_2);
-      r_1 <- k_3;
-      r_2 <- k_4;
-    } else {
-      
-    }
-    store_x2_last (output, plain, len, r_1, r_2);
-    return ();
-  }
-  
-  proc store_x8 (output:W64.t, plain:W64.t, len:W32.t, k_1:W32.t Array16.t,
-                 k_2:W32.t Array16.t, k_3:W32.t Array16.t,
-                 k_4:W32.t Array16.t, k_5:W32.t Array16.t,
-                 k_6:W32.t Array16.t, k_7:W32.t Array16.t,
-                 k_8:W32.t Array16.t) : W64.t * W64.t * W32.t = {
-    
-    
-    
-    (output, plain, len) <@ store (output, plain, len, k_1);
-    (output, plain, len) <@ store (output, plain, len, k_2);
-    (output, plain, len) <@ store (output, plain, len, k_3);
-    (output, plain, len) <@ store (output, plain, len, k_4);
-    (output, plain, len) <@ store (output, plain, len, k_5);
-    (output, plain, len) <@ store (output, plain, len, k_6);
-    (output, plain, len) <@ store (output, plain, len, k_7);
-    (output, plain, len) <@ store (output, plain, len, k_8);
-    return (output, plain, len);
-  }
-  
-  proc store_x8_last (output:W64.t, plain:W64.t, len:W32.t,
-                      k_1:W32.t Array16.t, k_2:W32.t Array16.t,
-                      k_3:W32.t Array16.t, k_4:W32.t Array16.t,
-                      k_5:W32.t Array16.t, k_6:W32.t Array16.t,
-                      k_7:W32.t Array16.t, k_8:W32.t Array16.t) : unit = {
-    
-    var r_1:W32.t Array16.t;
-    var r_2:W32.t Array16.t;
-    var r_3:W32.t Array16.t;
-    var r_4:W32.t Array16.t;
-    r_1 <- witness;
-    r_2 <- witness;
-    r_3 <- witness;
-    r_4 <- witness;
-    r_1 <- k_1;
-    r_2 <- k_2;
-    r_3 <- k_3;
-    r_4 <- k_4;
-    if (((W32.of_int 256) \ule len)) {
-      (output, plain, len) <@ store_x4 (output, plain, len, r_1, r_2, r_3,
-      r_4);
-      r_1 <- k_5;
-      r_2 <- k_6;
-      r_3 <- k_7;
-      r_4 <- k_8;
-    } else {
-      
-    }
-    store_x4_last (output, plain, len, r_1, r_2, r_3, r_4);
-    return ();
-  }
-  
-  proc increment_counter (st:W32.t Array16.t) : W32.t Array16.t = {
-    
-    
-    
-    st.[12] <- (st.[12] + (W32.of_int 8));
-    return (st);
-  }
-  
-  proc increment_counter_x8 (st_1:W32.t Array16.t, st_2:W32.t Array16.t,
-                             st_3:W32.t Array16.t, st_4:W32.t Array16.t,
-                             st_5:W32.t Array16.t, st_6:W32.t Array16.t,
-                             st_7:W32.t Array16.t, st_8:W32.t Array16.t) : 
-  W32.t Array16.t * W32.t Array16.t * W32.t Array16.t * W32.t Array16.t *
-  W32.t Array16.t * W32.t Array16.t * W32.t Array16.t * W32.t Array16.t = {
-    
-    
-    
-    st_1 <@ increment_counter (st_1);
-    st_2 <@ increment_counter (st_2);
-    st_3 <@ increment_counter (st_3);
-    st_4 <@ increment_counter (st_4);
-    st_5 <@ increment_counter (st_5);
-    st_6 <@ increment_counter (st_6);
-    st_7 <@ increment_counter (st_7);
-    st_8 <@ increment_counter (st_8);
-    return (st_1, st_2, st_3, st_4, st_5, st_6, st_7, st_8);
-  }
-  
-  proc line (k:W32.t Array16.t, a:int, b:int, c:int, r:int) : W32.t Array16.t = {
-    var aux_0: bool;
-    var aux: bool;
-    var aux_1: W32.t;
-    
-    var  _0:bool;
-    var  _1:bool;
-    
-    k.[a] <- (k.[a] + k.[b]);
-    k.[c] <- (k.[c] `^` k.[a]);
-    (aux_0, aux, aux_1) <- x86_ROL_32 k.[c] (W8.of_int r);
-     _0 <- aux_0;
-     _1 <- aux;
-    k.[c] <- aux_1;
-    return (k);
-  }
-  
-  proc quarter_round (k:W32.t Array16.t, a:int, b:int, c:int, d:int) : W32.t Array16.t = {  
-    k <@ line (k, a, b, d, 16);
-    k <@ line (k, c, d, b, 12);
-    k <@ line (k, a, b, d, 8);
-    k <@ line (k, c, d, b, 7);
-    return (k);
-  }
-  
-  proc rounds (k:W32.t Array16.t) : W32.t Array16.t = {
-    
-    var c:W32.t;
-    
-    c <- (W32.of_int 0);
-    
-    while ((c \ult (W32.of_int 10))) {
-      k <@ quarter_round (k, 0, 4, 8, 12);
-      k <@ quarter_round (k, 2, 6, 10, 14);
-      k <@ quarter_round (k, 1, 5, 9, 13);
-      k <@ quarter_round (k, 3, 7, 11, 15);
-      k <@ quarter_round (k, 1, 6, 11, 12);
-      k <@ quarter_round (k, 0, 5, 10, 15);
-      k <@ quarter_round (k, 2, 7, 8, 13);
-      k <@ quarter_round (k, 3, 4, 9, 14);
-      c <- (c + (W32.of_int 1));
-    }
-    return (k);
-  }
-  
-  proc round_x2_body (k_1:W32.t Array16.t, k_2:W32.t Array16.t) : W32.t Array16.t *
-                                                              W32.t Array16.t = {
-    (k_1, k_2) = column_round_x2(k, r16, r8);
-    (k_1, k_2) = diagonal_round_x2(k, r16, r8);
-    return (k_1, k_2);
-  }
-
-  proc rounds_x2_body (k_1:W32.t Array16.t, k_2:W32.t Array16.t) : W32.t Array16.t *
-                                                              W32.t Array16.t = {
-    var c : int;
-    c = 0;
-    while (c < 10) {
-      (k_1, k_2) <- round_x2(k_1, k_2);
-      c <- c + 1;
-    }
-    return (k_1, k_2);
-  }
-  
-  proc rounds_x4 (k_1:W32.t Array16.t, k_2:W32.t Array16.t,
-                  k_3:W32.t Array16.t, k_4:W32.t Array16.t) : W32.t Array16.t *
-                                                              W32.t Array16.t *
-                                                              W32.t Array16.t *
-                                                              W32.t Array16.t = {
-    
-    
-    
-    k_1 <@ rounds (k_1);
-    k_2 <@ rounds (k_2);
-    k_3 <@ rounds (k_3);
-    k_4 <@ rounds (k_4);
-    return (k_1, k_2, k_3, k_4);
-  }
-  
-  proc rounds_x8 (k_1:W32.t Array16.t, k_2:W32.t Array16.t,
-                  k_3:W32.t Array16.t, k_4:W32.t Array16.t,
-                  k_5:W32.t Array16.t, k_6:W32.t Array16.t,
-                  k_7:W32.t Array16.t, k_8:W32.t Array16.t) : W32.t Array16.t *
-                                                              W32.t Array16.t *
-                                                              W32.t Array16.t *
-                                                              W32.t Array16.t *
-                                                              W32.t Array16.t *
-                                                              W32.t Array16.t *
-                                                              W32.t Array16.t *
-                                                              W32.t Array16.t = {
-    
-    
-    
-    k_1 <@ rounds (k_1);
-    k_2 <@ rounds (k_2);
-    k_3 <@ rounds (k_3);
-    k_4 <@ rounds (k_4);
-    k_5 <@ rounds (k_5);
-    k_6 <@ rounds (k_6);
-    k_7 <@ rounds (k_7);
-    k_8 <@ rounds (k_8);
-    return (k_1, k_2, k_3, k_4, k_5, k_6, k_7, k_8);
-  }
-  
-  proc chacha20_more_than_256 (output:W64.t, plain:W64.t, len:W32.t,
-                               key:W64.t, nonce:W64.t, counter:W32.t) : unit = {
-    
-    var st_1:W32.t Array16.t;
-    var st_2:W32.t Array16.t;
-    var st_3:W32.t Array16.t;
-    var st_4:W32.t Array16.t;
-    var st_5:W32.t Array16.t;
-    var st_6:W32.t Array16.t;
-    var st_7:W32.t Array16.t;
-    var st_8:W32.t Array16.t;
-    var k_1:W32.t Array16.t;
-    var k_2:W32.t Array16.t;
-    var k_3:W32.t Array16.t;
-    var k_4:W32.t Array16.t;
-    var k_5:W32.t Array16.t;
-    var k_6:W32.t Array16.t;
-    var k_7:W32.t Array16.t;
-    var k_8:W32.t Array16.t;
-    k_1 <- witness;
-    k_2 <- witness;
-    k_3 <- witness;
-    k_4 <- witness;
-    k_5 <- witness;
-    k_6 <- witness;
-    k_7 <- witness;
-    k_8 <- witness;
-    st_1 <- witness;
-    st_2 <- witness;
-    st_3 <- witness;
-    st_4 <- witness;
-    st_5 <- witness;
-    st_6 <- witness;
-    st_7 <- witness;
-    st_8 <- witness;
-    (st_1, st_2, st_3, st_4, st_5, st_6, st_7, st_8) <@ init_x8 (key, nonce,
-    counter);
-    
-    while (((W32.of_int 512) \ule len)) {
-      (k_1, k_2, k_3, k_4, k_5, k_6, k_7, k_8) <@ copy_state_x8 (st_1, st_2,
-      st_3, st_4, st_5, st_6, st_7, st_8);
-      (k_1, k_2, k_3, k_4, k_5, k_6, k_7, k_8) <@ rounds_x8 (k_1, k_2, k_3,
-      k_4, k_5, k_6, k_7, k_8);
-      (k_1, k_2, k_3, k_4, k_5, k_6, k_7, k_8) <@ sum_states_x8 (k_1, k_2,
-      k_3, k_4, k_5, k_6, k_7, k_8, st_1, st_2, st_3, st_4, st_5, st_6, st_7,
-      st_8);
-      (output, plain, len) <@ store_x8 (output, plain, len, k_1, k_2, k_3,
-      k_4, k_5, k_6, k_7, k_8);
-      (st_1, st_2, st_3, st_4, st_5, st_6, st_7,
-      st_8) <@ increment_counter_x8 (st_1, st_2, st_3, st_4, st_5, st_6,
-      st_7, st_8);
-    }
-    if (((W32.of_int 0) \ult len)) {
-      (k_1, k_2, k_3, k_4, k_5, k_6, k_7, k_8) <@ copy_state_x8 (st_1, st_2,
-      st_3, st_4, st_5, st_6, st_7, st_8);
-      (k_1, k_2, k_3, k_4, k_5, k_6, k_7, k_8) <@ rounds_x8 (k_1, k_2, k_3,
-      k_4, k_5, k_6, k_7, k_8);
-      (k_1, k_2, k_3, k_4, k_5, k_6, k_7, k_8) <@ sum_states_x8 (k_1, k_2,
-      k_3, k_4, k_5, k_6, k_7, k_8, st_1, st_2, st_3, st_4, st_5, st_6, st_7,
-      st_8);
-      store_x8_last (output, plain, len, k_1, k_2, k_3, k_4, k_5, k_6, k_7,
-      k_8);
-    } else {
-      
-    }
-    return ();
-  }
-  
-  proc chacha20_less_than_257 (output:W64.t, plain:W64.t, len:W32.t,
-                               key:W64.t, nonce:W64.t, counter:W32.t) : unit = {
-    
-    var st_1:W32.t Array16.t;
-    var st_2:W32.t Array16.t;
-    var k1_1:W32.t Array16.t;
-    var k1_2:W32.t Array16.t;
-    var k2_1:W32.t Array16.t;
-    var k2_2:W32.t Array16.t;
-    k1_1 <- witness;
-    k1_2 <- witness;
-    k2_1 <- witness;
-    k2_2 <- witness;
-    st_1 <- witness;
-    st_2 <- witness;
-    (st_1, st_2) <@ init_x2 (key, nonce, counter);
-    if (((W32.of_int 128) \ult len)) {
-      (k1_1, k1_2, k2_1, k2_2) <@ copy_state_x4 (st_1, st_2);
-      (k1_1, k1_2, k2_1, k2_2) <@ rounds_x4 (k1_1, k1_2, k2_1, k2_2);
-      (k1_1, k1_2, k2_1, k2_2) <@ sum_states_x4 (k1_1, k1_2, k2_1, k2_2,
-      st_1, st_2);
-      (output, plain, len) <@ store_x2 (output, plain, len, k1_1, k1_2);
-      store_x2_last (output, plain, len, k2_1, k2_2);
-    } else {
-      (k1_1, k1_2) <@ copy_state_x2 (st_1, st_2);
-      (k1_1, k1_2) <@ rounds_x2 (k1_1, k1_2);
-      (k1_1, k1_2) <@ sum_states_x2 (k1_1, k1_2, st_1, st_2);
-      store_x2_last (output, plain, len, k1_1, k1_2);
-    }
-    return ();
-  }
-  
-  proc chacha20_avx2 (output:W64.t, plain:W64.t, len:W32.t, key:W64.t,
-                      nonce:W64.t, counter:W32.t) : unit = {
-    
-    
-    
-    if ((len \ult (W32.of_int 257))) {
-      chacha20_less_than_257 (output, plain, len, key, nonce, counter);
-    } else {
-      chacha20_more_than_256 (output, plain, len, key, nonce, counter);
-    }
-    return ();
-  }
-}.
 
